Lambda/TypedCombinators.v
@@ -3,7 +3,6 @@ Import ListNotations.
 
 Require Import FormalSystems.Base.
 
-
 (** * Types and terms *)
 
 Inductive Ty : Type :=
@@ -62,6 +61,8 @@ Inductive red : Tm -> Tm -> Prop :=
         forall t1 t2 t2' : Tm,
           red t2 t2' -> red (t1 @ t2) (t1 @ t2').
 
+Notation "A ~> B" := (red A B) (at level 60).
+
 Hint Constructors Ty Tm hasType red rtc : core.
 
 Definition reds := rtc red.
@@ -69,41 +70,222 @@ Definition reds := rtc red.
 Definition isNormal (t : Tm) : Prop :=
   forall t' : Tm, ~ red t t'.
 
+Inductive Nf : Tm -> Prop :=
+    | Nf_K0    : Nf K
+    | Nf_K1    : forall t : Tm, Nf t -> Nf (K @ t)
+    | Nf_S0    : Nf S
+    | Nf_S1    : forall t : Tm, Nf t -> Nf (S @ t)
+    | Nf_S2    : forall t1 t2 : Tm, Nf t1 -> Nf t2 -> Nf (S @ t1 @ t2)
+    | Nf_zero  : Nf zero
+    | Nf_succ0 : Nf succ
+    | Nf_succ1 : forall t : Tm, Nf t -> Nf (succ @ t)
+    | Nf_rec0  : Nf rec
+    | Nf_rec1  : forall t : Tm, Nf t -> Nf (rec @ t)
+    | Nf_rec2  : forall t1 t2 : Tm, Nf t1 -> Nf t2 -> Nf (rec @ t1 @ t2)
+    | Nf_Ne    : forall t : Tm, Ne t -> Nf t
+
+with Ne : Tm -> Prop :=
+    | Ne_App : forall t1 t2 : Tm, Ne t1 -> Nf t2 -> Ne (t1 @ t2)
+    | Ne_rec : forall t1 t2 t3 : Tm, Nf t1 -> Nf t2 -> Ne t3 -> Ne (rec @ t1 @ t2 @ t3).
+
+Inductive Nf' : Tm -> Prop :=
+    | Nf'App  : forall t1 t2 : Tm, Ne' t1 -> Nf' t2 -> Nf' (t1 @ t2)
+    | Nf'Ne'  : forall t : Tm, Ne' t -> Nf' t
+
+with      Ne' : Tm -> Prop :=
+    | Ne'K    : Ne' K
+    | Ne'S0   : Ne' S
+    | Ne'S1   : forall t : Tm, Nf' t -> Ne' (S @ t)
+    | Ne'zero : Ne' zero
+    | Ne'succ : Ne' succ
+    | Ne'rec0 : Ne' rec
+    | Ne'rec1 : forall t : Tm, Nf' t -> Ne' (rec @ t).
+
+Hint Constructors Nf Ne Nf' Ne' : core.
+
+Ltac wut :=
+repeat match goal with
+    | |- forall _, _ => intro
+    | |- ~ _ => intro
+    | |- _ /\ _ => split
+    | H : _ /\ _ |- _ => destruct H
+    | H : red (_ @ _) _ |- _ => inv H
+    | H : red K       _ |- _ => inv H
+    | H : red S       _ |- _ => inv H
+    | H : red zero    _ |- _ => inv H
+    | H : red succ    _ |- _ => inv H
+    | H : red rec     _ |- _ => inv H
+    | H : isNormal ?t, H' : red ?t _ |- _ => destruct (H _ H')
+    | |- isNormal _ => do 2 intro
+    | H : exists _, _   |- _ => decompose [ex and] H; clear H
+    | H : Ne ?x          |- _ => is_var x + inv H
+    | H : Ne' ?x          |- _ => is_var x + inv H
+    | _ => auto
+end.
+
+Fixpoint Nf_isNormal {t : Tm} (nf : Nf t) {struct nf} : isNormal t
+
+with     Ne_isNormal {t : Tm} (ne : Ne t) {struct ne} : isNormal t.
+Proof.
+  destruct nf.
+    1-11: wut; eapply Nf_isNormal;
+      repeat match goal with
+          | |- red _ _ => eauto
+      end; eauto.
+    apply Ne_isNormal. assumption.
+  destruct ne.
+    wut.
+      eapply Ne_isNormal; eauto.
+      eapply Nf_isNormal; eauto.
+    wut.
+      eapply Nf_isNormal. 2: eauto. eauto.
+      eapply Nf_isNormal. 2: eauto. eauto.
+      eapply Ne_isNormal. 2: eauto. eauto.
+Qed.
+
+Fixpoint Nf'_isNormal {t : Tm} (nf : Nf' t) {struct nf} : isNormal t
+
+with     Ne'_isNormal {t : Tm} (ne : Ne' t) {struct ne} : isNormal t.
+Proof.
+  destruct nf; wut.
+    eapply Ne'_isNormal; eauto.
+    eapply Nf'_isNormal; eauto.
+    eapply Ne'_isNormal; eauto.
+  destruct ne; wut.
+    eapply Nf'_isNormal; eauto.
+    eapply Nf'_isNormal; eauto.
+Qed.
+
+Lemma isNormal_Nf' :
+  forall t : Tm, isNormal t -> Nf' t.
+Proof.
+  unfold isNormal.
+  induction t; intros; auto.
+  destruct t1. all: cycle 3.
+    constructor; auto. apply IHt2. wut. eapply H. eauto.
+    constructor; auto. apply IHt2. wut. eapply H. eauto.
+    constructor; auto. apply IHt2. wut. eapply H. eauto.
+    constructor; auto. apply IHt2. wut. eapply H. eauto.
+    constructor; auto. apply IHt2. wut. eapply H. eauto.
+    destruct t1_1. all: cycle 3.
+      repeat constructor. auto.
+Abort.
+
 Definition hasNormal (t : Tm) : Prop :=
   exists t' : Tm, reds t t' /\ isNormal t'.
 
 Definition WN (t : Tm) (a : Ty) : Prop :=
   exists t' : Tm, hasType t' a /\ rtc red t t' /\ isNormal t'.
 
-(* Inductive Reducible : Tm -> Ty -> Prop :=
-    | Reducible_TNat :
-        forall t : Tm, WN t TNat -> Reducible t TNat
-    | Reducible_TArr :
-        forall (t : Tm) (a b : Ty),
-          WN t (TArr a b) ->
-          (forall t' : Tm, hasType t' a -> Reducible t' a -> Reducible (App t t') b) ->
-            Reducible t (TArr a b).
- *)
-
-Fixpoint Reducible (ty : Ty) (t : Tm) : Prop :=
+Fixpoint Reducible (t : Tm) (ty : Ty) : Prop :=
 match ty with
     | TNat     => WN t TNat
     | TArr a b => WN t (TArr a b) /\
                   forall t' : Tm,
-                    hasType t' a -> Reducible a t' -> Reducible b (App t t')
+                    hasType t' a -> Reducible t' a -> Reducible (t @ t') b
 end.
+
+Fixpoint R' (t : Tm) (ty : Ty) : Prop :=
+match ty with
+    | TNat     => True
+    | TArr a b => forall t' : Tm,
+                    hasType t' a -> R' t' a -> R' (t @ t') b
+end.
+
+Goal
+  forall t ty,
+    Reducible t ty <-> WN t ty /\ R' t ty.
+Proof.
+  split.
+    revert t. induction ty; cbn; intros.
+      auto.
+      firstorder. destruct ty2; cbn.
+        trivial.
+        intros. cbn in *. edestruct IHty2.
+Abort.
+
+Lemma reds_AppL :
+  forall t1 t1' t2 : Tm,
+    reds t1 t1' -> reds (t1 @ t2) (t1' @ t2).
+Proof.
+  unfold reds.
+  induction 1; eauto.
+Qed.
+
+Lemma reds_AppR :
+  forall t1 t2 t2' : Tm,
+    reds t2 t2' -> reds (t1 @ t2) (t1 @ t2').
+Proof.
+  unfold reds.
+  induction 1; eauto.
+Qed.
+
+Lemma reds_App :
+  forall t1 t1' t2 t2' : Tm,
+    reds t1 t1' -> reds t2 t2' -> reds (t1 @ t2) (t1' @ t2').
+Proof.
+  intros.
+  eapply rtc_trans.
+    apply reds_AppL. eassumption.
+    apply reds_AppR. eassumption.
+Qed.
 
 Lemma hasType_Reducible :
   forall {a : Ty} {t : Tm},
-    hasType t a -> Reducible a t.
+    hasType t a -> Reducible t a.
 Proof.
   induction 1.
     cbn. split.
-      red. exists K. repeat split; auto. red. do 2 intro. inv H.
+      red. exists K. repeat split; auto. wut.
       split; intros.
         red. destruct a; cbn in *; unfold WN in *.
           decompose [ex and] H0; clear H0. exists (K @ x). split; eauto. split.
-            admit. (* rtc_AppR *)
-            red. do 2 intro. inv H0.
-              inv H7.
+            apply reds_AppR. assumption.
+            wut.
+          decompose [ex and] H0; clear H0. exists (K @ x). split; eauto. split.
+            apply reds_AppR. assumption.
+            wut.
+        clear -a H0. induction a; cbn in *; unfold WN in *; intros.
+          wut. exists x. wut. constructor 3 with (K @ x @ t'0).
+            apply reds_AppL, reds_AppR. assumption.
+            auto.
+          wut.
+            exists x. wut. constructor 3 with (K @ x @ t'0).
+              apply reds_AppL, reds_AppR. assumption.
+              auto.
+            admit.
+    admit.
+    cbn in *. wut.
+    cbn. wut. red. exists zero. wut.
+    cbn. wut.
+      red. exists succ. wut.
+      unfold WN in *. wut. exists (succ @ x). wut.
+        eauto.
+        apply reds_AppR. assumption.
+    cbn. unfold WN. wut.
+      exists rec. wut.
+      destruct a; cbn in *; unfold WN in *; wut.
+        exists (rec @ x). wut.
+          eauto.
+          apply reds_AppR. assumption.
+        exists (rec @ x). wut.
+          eauto.
+          apply reds_AppR. assumption.
+      destruct a; cbn in *; unfold WN in *; wut.
+        exists (rec @ x0 @ x). wut.
+          eauto.
+          repeat apply reds_App; unfold reds; auto.
+        exists (rec @ x0 @ x). wut.
+          eauto.
+          repeat apply reds_App; unfold reds; auto.
+      edestruct (H5 _ H7).
+        exists x. wut.
+        wut. destruct a; cbn.
+Restart.
+  induction a; cbn; intros.
+    red. remember TNat as n. revert Heqn. induction H; inversion 1; subst.
+      admit.
+      admit.
+    wut.
+      red. exists t. wut.
 Abort.
